Add files via upload

Mutex.thy
@@ -30,14 +30,13 @@ record 'a mutex =
  local1    :: "'a"
  
  
-definition "inv0 s \<equiv> turn_aux0 s \<longrightarrow> flag0 s \<longrightarrow> turn s"
+definition "cond0 s \<equiv> turn_aux1 s \<longrightarrow> flag1 s \<longrightarrow> \<not>turn s"
   
-definition "inv1 s \<equiv> turn_aux1 s \<longrightarrow> flag1 s \<longrightarrow> \<not> turn s"
+definition "cond1 s \<equiv> turn_aux0 s \<longrightarrow> flag0 s \<longrightarrow> turn s"
    
-    
 
     
-section "The model with auxiliaries"    
+subsection "The model with auxiliaries"    
 
 definition 
 "thread0_aux cs P \<equiv>
@@ -66,8 +65,8 @@ definition
 "mutex_aux P0 cs0 Q0 P1 cs1 Q1 \<equiv>
    INTERLEAVING-BEGIN
     \<lbrakk> rely: \<lbrace> \<ordmasculine>flag0 = \<ordfeminine>flag0 \<and> \<ordmasculine>turn_aux0 = \<ordfeminine>turn_aux0 \<and> \<ordmasculine>local0 = \<ordfeminine>local0 \<and>
-             (\<ordmasculine>turn_aux0 \<longrightarrow> \<ordmasculine>flag0 \<longrightarrow> \<ordmasculine>inv1 \<longrightarrow> \<ordmasculine>shared = \<ordfeminine>shared) \<and>
-             (\<ordmasculine>inv1 \<longrightarrow> \<ordfeminine>inv1) \<and>
+             (\<ordmasculine>turn_aux0 \<longrightarrow> \<ordmasculine>flag0 \<longrightarrow> \<ordmasculine>cond0 \<longrightarrow> \<ordmasculine>shared = \<ordfeminine>shared) \<and>
+             (\<ordmasculine>cond0 \<longrightarrow> \<ordfeminine>cond0) \<and>
              (P0 \<ordmasculine>shared \<longrightarrow> P0 \<ordfeminine>shared) \<and> (Q0 \<ordmasculine>shared \<longrightarrow> Q0 \<ordfeminine>shared) \<rbrace>,
       pre:  \<lbrace> \<not>\<acute>turn_aux0 \<and> P0 \<acute>shared \<rbrace>,
       post: \<lbrace>  Q0 \<acute>shared \<rbrace> 
@@ -75,8 +74,8 @@ definition
     thread0_aux cs0 P0 
   \<parallel>
     \<lbrakk> rely: \<lbrace> \<ordmasculine>flag1 = \<ordfeminine>flag1 \<and> \<ordmasculine>turn_aux1 = \<ordfeminine>turn_aux1 \<and> \<ordmasculine>local1 = \<ordfeminine>local1 \<and>
-             (\<ordmasculine>turn_aux1 \<longrightarrow> \<ordmasculine>flag1 \<longrightarrow> \<ordmasculine>inv0 \<longrightarrow> \<ordmasculine>shared = \<ordfeminine>shared) \<and>
-             (\<ordmasculine>inv0 \<longrightarrow> \<ordfeminine>inv0) \<and> 
+             (\<ordmasculine>turn_aux1 \<longrightarrow> \<ordmasculine>flag1 \<longrightarrow> \<ordmasculine>cond1 \<longrightarrow> \<ordmasculine>shared = \<ordfeminine>shared) \<and>
+             (\<ordmasculine>cond1 \<longrightarrow> \<ordfeminine>cond1) \<and> 
              (P1 \<ordmasculine>shared \<longrightarrow> P1 \<ordfeminine>shared) \<and> (Q1 \<ordmasculine>shared \<longrightarrow> Q1 \<ordfeminine>shared) \<rbrace>,
      pre:  \<lbrace> \<not>\<acute>turn_aux1 \<and> P1 \<acute>shared \<rbrace>,
      post: \<lbrace>  Q1 \<acute>shared \<rbrace>
@@ -85,8 +84,8 @@ definition
    INTERLEAVING-END" 
 
 
-section "The model without auxiliaries"    
 
+subsection "The model without auxiliaries"    
 
 definition 
 "thread0 cs \<equiv>
@@ -120,7 +119,7 @@ definition
 section "Properties"
   
 definition "mutexR0 = {((s :: ('a, 'b) mutex_scheme), (t :: ('a, 'b) mutex_scheme)). 
-                       turn_aux0 t \<and> flag0 t \<and> inv1 t \<and> s = t}"  
+                       turn_aux0 t \<and> flag0 t \<and> cond0 t \<and> s = t}"  
 
 lemma thread0_aux:
 " \<rho> \<Turnstile> cs0 
@@ -135,38 +134,38 @@ lemma thread0_aux:
 
  \<rho> \<Turnstile> thread0_aux cs0 P0 
  RELY \<lbrace> \<ordmasculine>flag0 = \<ordfeminine>flag0 \<and> \<ordmasculine>turn_aux0 = \<ordfeminine>turn_aux0 \<and> \<ordmasculine>local0 = \<ordfeminine>local0 \<and>
-        (\<ordmasculine>turn_aux0 \<longrightarrow> \<ordmasculine>flag0 \<longrightarrow> \<ordmasculine>inv1 \<longrightarrow> \<ordmasculine>shared = \<ordfeminine>shared) \<and>
-        (\<ordmasculine>inv1 \<longrightarrow> \<ordfeminine>inv1) \<and> 
+        (\<ordmasculine>turn_aux0 \<longrightarrow> \<ordmasculine>flag0 \<longrightarrow> \<ordmasculine>cond0 \<longrightarrow> \<ordmasculine>shared = \<ordfeminine>shared) \<and>
+        (\<ordmasculine>cond0 \<longrightarrow> \<ordfeminine>cond0) \<and> 
         (P0 \<ordmasculine>shared \<longrightarrow> P0 \<ordfeminine>shared) \<and> (Q0 \<ordmasculine>shared \<longrightarrow> Q0 \<ordfeminine>shared)  \<rbrace>
   PRE  \<lbrace> \<not>\<acute>turn_aux0 \<and> P0 \<acute>shared \<rbrace> 
   POST \<lbrace> Q0 \<acute>shared \<rbrace>
  GUAR \<lbrace> \<ordmasculine>flag1 = \<ordfeminine>flag1 \<and> \<ordmasculine>turn_aux1 = \<ordfeminine>turn_aux1 \<and> \<ordmasculine>local1 = \<ordfeminine>local1 \<and>
-        (\<ordmasculine>turn_aux1 \<longrightarrow> \<ordmasculine>flag1 \<longrightarrow> \<ordmasculine>inv0 \<longrightarrow> \<ordmasculine>shared = \<ordfeminine>shared) \<and>
-        (\<ordmasculine>inv0 \<longrightarrow> \<ordfeminine>inv0) \<and> 
+        (\<ordmasculine>turn_aux1 \<longrightarrow> \<ordmasculine>flag1 \<longrightarrow> \<ordmasculine>cond1 \<longrightarrow> \<ordmasculine>shared = \<ordfeminine>shared) \<and>
+        (\<ordmasculine>cond1 \<longrightarrow> \<ordfeminine>cond1) \<and> 
         (P1 \<ordmasculine>shared \<longrightarrow> P1 \<ordfeminine>shared) \<and> (Q1 \<ordmasculine>shared \<longrightarrow> Q1 \<ordfeminine>shared)  \<rbrace>"
   unfolding thread0_aux_def
   apply rg_tac
-     apply(simp (no_asm) add: inv0_def)
+     apply(simp (no_asm) add: cond1_def)
     apply(erule prog_corr_RG, assumption)
        apply(thin_tac _)+
        apply clarsimp
        apply(rename_tac s t t')
        apply(clarsimp simp: mutexR0_def)
        apply(rule_tac b=t' in relcompI, simp, simp)
-      apply(clarsimp simp: mutexR0_def inv1_def)
+      apply(clarsimp simp: mutexR0_def cond0_def)
      apply(clarsimp simp: mutexR0_def) 
-     apply(simp (no_asm) add: inv0_def)
+     apply(simp (no_asm) add: cond1_def)
     apply(thin_tac _)+
     apply(clarsimp simp: mutexR0_def)
     apply(rule conjI)
-     apply(simp add: inv0_def inv1_def)
-    apply(simp add: inv0_def)+
+     apply(simp add: cond0_def cond1_def)
+    apply(simp add: cond1_def)+
   done
 
     
 
 definition "mutexR1 = {((s :: ('a, 'b) mutex_scheme), (t :: ('a, 'b) mutex_scheme)). 
-                       s = t \<and> turn_aux1 t \<and> flag1 t \<and> inv0 t}"  
+                       s = t \<and> turn_aux1 t \<and> flag1 t \<and> cond1 t}"  
     
 lemma thread1_aux:
 " \<rho> \<Turnstile> cs1 
@@ -181,32 +180,32 @@ lemma thread1_aux:
 
  \<rho> \<Turnstile> thread1_aux cs1 P1 
  RELY \<lbrace> \<ordmasculine>flag1 = \<ordfeminine>flag1 \<and> \<ordmasculine>turn_aux1 = \<ordfeminine>turn_aux1 \<and> \<ordmasculine>local1 = \<ordfeminine>local1 \<and>
-        (\<ordmasculine>turn_aux1 \<longrightarrow> \<ordmasculine>flag1 \<longrightarrow> \<ordmasculine>inv0 \<longrightarrow> \<ordmasculine>shared = \<ordfeminine>shared) \<and>
-        (\<ordmasculine>inv0 \<longrightarrow> \<ordfeminine>inv0) \<and> 
+        (\<ordmasculine>turn_aux1 \<longrightarrow> \<ordmasculine>flag1 \<longrightarrow> \<ordmasculine>cond1 \<longrightarrow> \<ordmasculine>shared = \<ordfeminine>shared) \<and>
+        (\<ordmasculine>cond1 \<longrightarrow> \<ordfeminine>cond1) \<and> 
         (P1 \<ordmasculine>shared \<longrightarrow> P1 \<ordfeminine>shared) \<and> (Q1 \<ordmasculine>shared \<longrightarrow> Q1 \<ordfeminine>shared)  \<rbrace> 
   PRE  \<lbrace> \<not>\<acute>turn_aux1 \<and> P1 \<acute>shared \<rbrace> 
   POST \<lbrace> Q1 \<acute>shared \<rbrace> 
   GUAR \<lbrace> \<ordmasculine>flag0 = \<ordfeminine>flag0 \<and> \<ordmasculine>turn_aux0 = \<ordfeminine>turn_aux0 \<and> \<ordmasculine>local0 = \<ordfeminine>local0 \<and>
-        (\<ordmasculine>turn_aux0 \<longrightarrow> \<ordmasculine>flag0 \<longrightarrow> \<ordmasculine>inv1 \<longrightarrow> \<ordmasculine>shared = \<ordfeminine>shared) \<and>
-        (\<ordmasculine>inv1 \<longrightarrow> \<ordfeminine>inv1) \<and> 
+        (\<ordmasculine>turn_aux0 \<longrightarrow> \<ordmasculine>flag0 \<longrightarrow> \<ordmasculine>cond0 \<longrightarrow> \<ordmasculine>shared = \<ordfeminine>shared) \<and>
+        (\<ordmasculine>cond0 \<longrightarrow> \<ordfeminine>cond0) \<and> 
         (P0 \<ordmasculine>shared \<longrightarrow> P0 \<ordfeminine>shared) \<and> (Q0 \<ordmasculine>shared \<longrightarrow> Q0 \<ordfeminine>shared)  \<rbrace>"
   unfolding thread1_aux_def
   apply rg_tac
-     apply(simp (no_asm) add: inv1_def)
+     apply(simp (no_asm) add: cond0_def)
     apply(erule prog_corr_RG, assumption)
        apply(thin_tac _)+
        apply clarsimp
        apply(rename_tac s t t')
        apply(clarsimp simp: mutexR1_def)
        apply(rule_tac b=t' in relcompI, simp, simp)
-      apply(clarsimp simp: mutexR1_def inv0_def)
+      apply(clarsimp simp: mutexR1_def cond1_def)
      apply(clarsimp simp: mutexR1_def) 
-     apply(simp (no_asm) add: inv1_def)
+     apply(simp (no_asm) add: cond0_def)
     apply(thin_tac _)+
     apply(clarsimp simp: mutexR1_def)
     apply(rule conjI)
-     apply(simp add: inv0_def inv1_def)
-    apply(simp add: inv1_def)+
+     apply(simp add: cond0_def cond1_def)
+    apply(simp add: cond0_def)+
   done
 
 
@@ -352,7 +351,8 @@ lemma concurrent_upds[simplified] :
   apply(rule mutex)
        apply(simp, rule shared_upd0)
       apply(simp, rule shared_upd1)
-     apply(simp_all add: shared_upd0_def shared_upd1_def mutexR0_def mutexR1_def mutexR_def inv0_def inv1_def)
+     apply(simp_all add: shared_upd0_def shared_upd1_def mutexR0_def mutexR1_def mutexR_def 
+           cond0_def cond1_def)
      apply plain_prog_corr_tac+
   done
 
